src/Distributions/Uniform/Model.dfy
@@ -6,7 +6,7 @@
 module Uniform.Model {
   import Measures
   import Helper
-  import Random
+  import Rand
   import Quantifier
   import Monad
   import Independence
@@ -36,7 +36,7 @@ module Uniform.Model {
   function IntervalSample(a: int, b: int): (f: Monad.Hurd<int>)
     requires a < b
   {
-    (s: Random.Bitstream) =>
+    (s: Rand.Bitstream) =>
       var (x, s') := Sample(b - a)(s);
       (a + x, s')
   }
@@ -52,25 +52,25 @@ module Uniform.Model {
       UniformPowerOfTwo.Correctness.SampleIsIndep(2 * n);
     }
     var e := iset s | Loops.ProposalIsAccepted(Proposal(n), Accept(n))(s);
-    assert e in Random.eventSpace by {
+    assert e in Rand.eventSpace by {
       assert e == Measures.PreImage(s => UniformPowerOfTwo.Model.Sample(2 * n)(s).0, (iset m: nat | m < n));
-      assert Measures.PreImage(s => UniformPowerOfTwo.Model.Sample(2 * n)(s).0, (iset m: nat | m < n)) in Random.eventSpace by {
+      assert Measures.PreImage(s => UniformPowerOfTwo.Model.Sample(2 * n)(s).0, (iset m: nat | m < n)) in Rand.eventSpace by {
         assert Independence.IsIndep(UniformPowerOfTwo.Model.Sample(2 * n)) by {
           UniformPowerOfTwo.Correctness.SampleIsIndep(2 * n);
         }
-        assert Measures.IsMeasurable(Random.eventSpace, Measures.natEventSpace, s => UniformPowerOfTwo.Model.Sample(2 * n)(s).0) by {
+        assert Measures.IsMeasurable(Rand.eventSpace, Measures.natEventSpace, s => UniformPowerOfTwo.Model.Sample(2 * n)(s).0) by {
           Independence.IsIndepImpliesFstMeasurableNat(UniformPowerOfTwo.Model.Sample(2 * n));
         }
       }
     }
     assert Quantifier.WithPosProb(Loops.ProposalIsAccepted(Proposal(n), Accept(n))) by {
-      assert Random.prob(e) > 0.0 by {
+      assert Rand.prob(e) > 0.0 by {
         assert e == (iset s | UniformPowerOfTwo.Model.Sample(2 * n)(s).0 < n);
         assert n <= Helper.Power(2, Helper.Log2Floor(2 * n)) by {
           Helper.NLtPower2Log2FloorOf2N(n);
         }
         calc {
-          Random.prob(e);
+          Rand.prob(e);
         == { UniformPowerOfTwo.Correctness.UnifCorrectness2Inequality(2 * n, n); }
           n as real / (Helper.Power(2, Helper.Log2Floor(2 * n)) as real);
         >
